---
title: "Binomische Formeln"
---

Achtung: $(a+b)^2 \neq a^2 + b^2$.^[... wenn nicht gerade $a=0$ oder $b=0$.] Es gilt nämlich

\begin{equation}
(a+b)^2 = a^2+2ab+b^2, (\#eq:binom1)
\end{equation}

\begin{equation}
(a-b)^2 = a^2-2ab+b^2,(\#eq:binom2)
\end{equation}

\begin{equation}
(a+b)(a-b) = a^2-b^2. (\#eq:binom3)
\end{equation}

::: {.callout-caution collapse="true"}
## Kannst du die erste Formel durch Ausmultiplizieren überprüfen?

\begin{align*}
(a+b)^2 &= (a+b)(a+b) = a(a+b) + b(a+b) \\ &= a^2 + ab + ba + b^2 = a^2 + 2ab + b^2
\end{align*}
:::
